root_active.v
@@ -258,6 +258,70 @@ Proof.
   - intro; autorewrite with shints; repeat ysplit; pose_term_eq; csolve.
 Qed.
 
+Lemma lem_subst0_step : forall t s, step_beta t s ->
+                                    forall n t0, t == t0 [n := var 0] ->
+                                                 exists s0, s == s0 [n := var 0] /\ step_beta t0 s0.
+Proof.
+  induction 1.
+  - inversion_clear H; intros.
+    rewrite H in *; clear H.
+    inversion H0; subst; yisolve; fold term_eq in *.
+    destruct t0; autorewrite with shints in *; sauto.
+    destruct t0_1; autorewrite with shints in *; try yelles 1.
+    inversion H4; yisolve; fold term_eq in *.
+    exists (t0_1 [0 := t0_2]).
+    split.
+    + generalize (lem_subst_eq n 0 (var 0) t0_1 t0_2); autorewrite with yhints; intro HH.
+      rewrite HH.
+      rewrite H3.
+      rewrite H5.
+      assumption.
+    + Reconstr.reasy (lem_step_beta_redex) Reconstr.Empty.
+  - intros.
+    inversion H1; subst; yisolve; fold term_eq in *.
+    destruct t0; autorewrite with shints in *; sauto.
+    generalize (IHcomp_clos n t0_1 H5); intro HH; destruct HH as [s0 [HH1 HH2]].
+    exists (app s0 t0_2).
+    rewrite <- H0.
+    rewrite HH1.
+    autorewrite with shints.
+    pose_term_eq; ycrush.
+  - intros.
+    inversion H1; subst; yisolve; fold term_eq in *.
+    destruct t0; autorewrite with shints in *; sauto.
+    generalize (IHcomp_clos n t0_2 H6); intro HH; destruct HH as [s0 [HH1 HH2]].
+    exists (app t0_1 s0).
+    rewrite <- H0.
+    rewrite HH1.
+    autorewrite with shints.
+    pose_term_eq; ycrush.
+  - intros.
+    destruct t0; autorewrite with shints in *; sauto.
+    inversion H0; subst; yisolve; fold term_eq in *.
+    generalize (IHcomp_clos (n + 1) t0 H3); intro HH; destruct HH as [s0 [HH1 HH2]].
+    exists (abs s0).
+    rewrite HH1.
+    autorewrite with shints.
+    pose_term_eq; ycrush.
+Qed.
+
+Lemma lem_subst0_red : forall t s, red_beta t s ->
+                                   forall n t0, t == t0 [n := var 0] ->
+                                                exists s0, s == s0 [n := var 0] /\ red_beta t0 s0.
+Proof.
+  induction 1; pose_red_beta; pose_term_eq; pose lem_subst0_step; ycrush.
+Qed.
+
+Lemma lem_subst0_rnf : forall t, is_rnf t -> forall n t0, t == t0 [n := var 0] -> is_rnf t0.
+Proof.
+  destruct t; sauto; destruct t0; autorewrite with shints in *; sauto.
+  destruct z; sauto.
+  inversion_clear H0; yisolve; fold term_eq in *.
+  assert (red_beta t1 ((abs x) [n := var 0])) by (pose lem_red_beta_subst_closed; ycrush).
+  autorewrite with shints in *.
+  pose_inf_beta; ycrush.
+Qed.
+
 Lemma lem_has_rnf_subst : forall n t1 t2, has_rnf (t1 [n := t2]) -> has_rnf t1.
 Proof.
   unfold has_rnf.
@@ -271,5 +335,246 @@ Proof.
   sauto.
   assert (is_rnf s1) by
       Reconstr.reasy (@lem_succ_preserves_rnf) (@defs.is_rnf).
-  admit.
-Admitted.
+  assert (exists s0, s1 == s0 [n := var 0] /\ red_beta t1 s0) by
+      (pose lem_subst0_red; pose_term_eq; ycrush).
+  sauto.
+  assert (is_rnf s0) by
+      Reconstr.reasy (@lem_subst0_rnf) (@defs.is_rnf).
+  Reconstr.reasy (lem_red_beta_to_inf_beta) Reconstr.Empty.
+Qed.
+
+Lemma lem_is_rnf_shift : forall d c t, is_rnf (shift d c t) -> is_rnf t.
+Proof.
+  unfold is_rnf; sauto.
+  generalize lem_inf_beta_shift_closed; unfold shift_closed; ycrush.
+Qed.
+
+Lemma lem_is_rnf_morphism : forall x y, x == y -> is_rnf x -> is_rnf y.
+Proof.
+  intros x y H1 H2; destruct x, y; sauto.
+  inversion_clear H1; yisolve; fold term_eq in *.
+  rewrite <- H3 in H; ycrush.
+Qed.
+
+Add Parametric Morphism : is_rnf  with
+    signature term_eq ==> iff as is_rnf_mor.
+Proof.
+  pose lem_is_rnf_morphism; pose_term_eq; ycrush.
+Qed.
+
+Lemma lem_has_rnf_shift : forall d c t, has_rnf (shift d c t) -> has_rnf t.
+Proof.
+  unfold has_rnf.
+  sauto.
+  assert (exists s, is_rnf s /\ red_beta (shift d c t) s) by
+      Reconstr.reasy (@weak.lem_rnf_red_wh, @weak.lem_red_wh_to_red_beta) Reconstr.Empty.
+  sauto.
+  assert (exists s', s == shift d c s' /\ red_beta t s') by
+      (pose lem_red_beta_shift; pose_term_eq; ycrush).
+  sauto.
+  exists s'.
+  split.
+  - rewrite H3 in H1; pose lem_is_rnf_shift; ycrush.
+  - pose_inf_beta; ycrush.
+Qed.
+
+Lemma lem_ra_subst : forall n t1 t2, root_active t1 -> root_active (t1 [n := t2]).
+Proof.
+  Reconstr.reasy (@lem_has_rnf_subst) (root_active).
+Qed.
+
+Lemma lem_ra_shift : forall d c t, root_active t -> root_active (shift d c t).
+Proof.
+  Reconstr.reasy (@lem_has_rnf_shift) (@defs.root_active).
+Qed.
+
+Definition sim_ra := sim root_active.
+Hint Unfold sim_ra.
+
+Lemma lem_sim_ra_shift : forall n m t t', sim_ra t t' ->
+                                          sim_ra (shift n m t) (shift n m t').
+Proof.
+  pose lem_ra_shift; coinduction.
+Qed.
+
+Lemma lem_sim_ra_subst : forall n t t' s s', sim_ra t t' -> sim_ra s s' ->
+                                             sim_ra (t [n := s]) (t' [n := s']).
+Proof.
+  pose lem_ra_subst; pose lem_sim_ra_shift; coinduction.
+Qed.
+
+Lemma lem_inf_beta_preserves_ra : forall t s, inf_beta t s -> root_active t -> root_active s.
+Proof.
+  unfold root_active; unfold has_rnf; pose_inf_beta; ycrush.
+Qed.
+
+Lemma lem_ra_morphism : forall t s, t == s -> root_active t -> root_active s.
+Proof.
+  unfold root_active; unfold has_rnf; pose_term_eq; ycrush.
+Qed.
+
+Lemma lem_sim_ra_morphism : morphism sim_ra.
+Proof.
+  unfold morphism.
+  coinduction CH.
+  - clear CH; pose lem_ra_morphism; pose_term_eq; ycrush.
+  - intros.
+    destruct x'0, y'0; try solve [ clear CH; yelles 1 ].
+    inversion_clear H2; yisolve.
+    inversion_clear H3; yisolve.
+    fold term_eq in *.
+    constructor 4.
+    eapply CH with (x := x0) (y := x'); clear CH; pose_term_eq; ycrush.
+    eapply CH with (x := y0) (y := y'); clear CH; pose_term_eq; ycrush.
+Qed.
+
+Add Parametric Morphism : sim_ra  with
+    signature term_eq ==> term_eq ==> iff as sim_ra_mor.
+Proof.
+  pose lem_sim_ra_morphism; pose_term_eq; ycrush.
+Qed.
+
+Lemma lem_ra_not_abs : forall x, ~(root_active (abs x)).
+Proof.
+  unfold root_active, not, has_rnf; pose_inf_beta; ycrush.
+Qed.
+
+Lemma lem_ra_not_var : forall n, ~(root_active (var n)).
+Proof.
+  unfold root_active, not, has_rnf; pose_inf_beta; ycrush.
+Qed.
+
+Lemma lem_step_beta_preserves_sim_ra :
+  forall t t', step_beta t t' -> forall s, sim_ra t s -> exists s', step_beta_eq s s' /\ sim_ra t' s'.
+Proof.
+  induction 1.
+  - intros s HH.
+    inversion HH; subst.
+    + exists s.
+      assert (inf_beta x y) by
+          Reconstr.rcrush (lem_step_beta_to_inf_beta, @defs.wh_base) Reconstr.Empty.
+      pose lem_inf_beta_preserves_ra; pose_term_eq; ycrush.
+    + sauto.
+    + sauto.
+    + inversion_clear H.
+      inversion H2; subst; yisolve; fold term_eq in *.
+      destruct x0; sauto.
+      inversion H6; subst; yisolve; fold term_eq in *.
+      inversion H0; subst; yisolve; fold term_eq in *.
+      * pose lem_ra_not_abs; ycrush.
+      * rewrite H8 in *.
+        rewrite H5 in *.
+        assert (sim_ra (t1 [0 := t2]) (y1 [0 := y'])) by
+            (pose lem_sim_ra_subst; ycrush).
+        exists (y1 [0 := y']).
+        rewrite H3.
+        Reconstr.reasy (@beta.lem_step_beta_redex) (@step_beta_eq).
+    + scrush.
+  - intros s HH.
+    rewrite H0 in *; clear H0 y.
+    inversion HH; subst.
+    + exists s.
+      assert (inf_beta (app x y') (app x' y')) by
+          Reconstr.reasy (@beta.lem_step_beta_to_red_beta, @beta.lem_red_beta_to_inf_beta, @beta.lem_inf_beta_app, @equality.lem_term_eq_refl, @beta.lem_red_beta_refl) (@defs.term_eq, @defs.step_beta, @Coq.Relations.Relation_Definitions.reflexive).
+      pose lem_inf_beta_preserves_ra; pose_term_eq; ycrush.
+    + generalize (IHcomp_clos x'0 H2); sauto.
+      exists (app s' y'0).
+      unfold step_beta_eq in *; pose_term_eq; ycrush.
+  - intros s HH.
+    rewrite H0 in *; clear H0 x.
+    inversion HH; subst.
+    + exists s.
+      assert (inf_beta (app x' y) (app x' y')) by
+          Reconstr.reasy (@beta.lem_step_beta_to_red_beta, @beta.lem_red_beta_to_inf_beta, @beta.lem_inf_beta_app, @equality.lem_term_eq_refl, @beta.lem_red_beta_refl) (@defs.term_eq, @defs.step_beta, @Coq.Relations.Relation_Definitions.reflexive).
+      pose lem_inf_beta_preserves_ra; pose_term_eq; ycrush.
+    + generalize (IHcomp_clos y'0 H4); sauto.
+      exists (app x'0 s').
+      unfold step_beta_eq in *; pose_term_eq; ycrush.
+  - intros s HH.
+    inversion HH; subst.
+    + Reconstr.reasy (@lem_ra_not_abs) Reconstr.Empty.
+    + generalize (IHcomp_clos y0 H1); sauto.
+      exists (abs s').
+      unfold step_beta_eq in *; pose_term_eq; ycrush.
+Qed.
+
+Lemma lem_red_beta_preserves_sim_ra :
+  forall t t', red_beta t t' -> forall s, sim_ra t s -> exists s', red_beta s s' /\ sim_ra t' s'.
+Proof.
+  induction 1.
+  - intros; rewrite H in *; unfold step_beta_eq; pose_term_eq; ycrush.
+  - intros.
+    generalize (lem_step_beta_preserves_sim_ra x y H s H1); sauto.
+    generalize (IHstar s' H3); sauto.
+    destruct H2; pose_red_beta; pose_term_eq; ycrush.
+Qed.
+
+Lemma lem_sim_ra_preserves_rnf : forall t s, sim_ra t s -> is_rnf t -> is_rnf s.
+Proof.
+  intros.
+  assert (~(root_active t)) by
+      Reconstr.reasy (@weak.lem_inf_wh_to_inf_beta, @weak.lem_inf_wh_refl_0) (@defs.inf_wh, @defs.has_rnf, @defs.root_active, @Coq.Relations.Relation_Definitions.reflexive).
+  destruct t; sauto.
+  - pose lem_ra_not_var; scrush.
+  - inversion H; sauto.
+    destruct z; sauto.
+    assert (HH: sim_ra x' t1) by (pose_sim; ycrush).
+    generalize (lem_red_beta_preserves_sim_ra x' (abs x) H5 t1 HH); sauto.
+    apply H0 with (z := s').
+    + pose_inf_beta; ycrush.
+    + destruct s'; pose lem_ra_not_abs; sauto.
+  - inversion H; sauto.
+Qed.
+
+Lemma lem_sim_ra_preserves_ra : forall t s, sim_ra t s -> root_active t -> root_active s.
+Proof.
+  unfold root_active, not, has_rnf.
+  sauto.
+  apply H0; clear H0.
+  assert (exists s', is_rnf s' /\ red_beta s s') by
+      Reconstr.reasy (@weak.lem_rnf_red_wh, @weak.lem_red_wh_to_red_beta) Reconstr.Empty.
+  sauto.
+  assert (sim_ra s t) by (pose_sim; ycrush).
+  assert (exists t0, red_beta t t0 /\ sim_ra s' t0) by
+      (pose lem_red_beta_preserves_sim_ra; ycrush).
+  pose_inf_beta; pose lem_sim_ra_preserves_rnf; ycrush.
+Qed.
+
+Lemma lem_ra_expansion : forall t s, inf_beta t s -> root_active s -> root_active t.
+Proof.
+  unfold root_active, not, has_rnf.
+  sauto.
+  apply H0; clear H0.
+  assert (exists t0, is_rnf t0 /\ red_wh t t0) by
+      Reconstr.reasy (@weak.lem_rnf_red_wh) Reconstr.Empty.
+  sauto.
+  assert (exists r, red_wh s r /\ inf_beta t0 r) by
+      Reconstr.rblast (@weak.lem_rnf_red_wh, @beta.lem_inf_beta_prepend, @weak.lem_inf_wh_to_inf_beta, @weak.lem_wh_commute, @weak.lem_inf_beta_to_inf_wh) (@defs.has_rnf).
+  sauto.
+  assert (is_rnf r) by
+      Reconstr.reasy (@beta.lem_inf_beta_preserves_rnf) Reconstr.Empty.
+  exists r.
+  Reconstr.reasy (@beta.lem_red_beta_to_inf_beta, @weak.lem_red_wh_to_inf_wh, @weak.lem_inf_wh_to_inf_beta) Reconstr.Empty.
+Qed.
+
+Theorem thm_ra_strongly_meaningless : strongly_meaningless root_active.
+Proof.
+  unfold strongly_meaningless, meaningless.
+  repeat split.
+  - unfold root_active, not, has_rnf.
+    sauto.
+    destruct t'; sauto.
+    + assert (bot == var n) by (pose lem_red_beta_preserves_bot; pose_term_eq; ycrush).
+      scrush.
+    + assert (bot == app x y) by (pose lem_red_beta_preserves_bot; pose_term_eq; ycrush).
+      scrush.
+    + assert (bot == abs x) by (pose lem_red_beta_preserves_bot; pose_term_eq; ycrush).
+      scrush.
+  - Reconstr.reasy (@lem_inf_beta_preserves_ra) Reconstr.Empty.
+  - Reconstr.reasy (@lem_ra_subst) Reconstr.Empty.
+  - Reconstr.reasy (@lem_ra_shift) Reconstr.Empty.
+  - Reconstr.reasy (@lem_ra_not_abs) Reconstr.Empty.
+  - auto.
+  - Reconstr.reasy (@lem_sim_ra_preserves_ra) (@sim_ra, @defs.has_rnf, @defs.is_rnf, @defs.root_active).
+  - Reconstr.reasy (@lem_ra_expansion) Reconstr.Empty.
+Qed.
